stuff

BlockCacheSystem/JournalInterval.i.dfy
@@ -4,7 +4,9 @@ include "DiskLayout.i.dfy"
 module JournalIntervals {
   import opened DiskLayout
   import opened JournalRanges
+  import opened Journal
   import opened Options
+  import opened Sequences
 
   datatype JournalInterval = JournalInterval(start: int, len: int)
 
@@ -25,7 +27,7 @@ module JournalIntervals {
     |journal| == NumJournalBlocks() as int
   }
 
-  function CyclicSliceValue(
+  function CyclicSpliceValue(
     journal: seq<Option<JournalBlock>>,
     indices: JournalInterval,
     newEntries: seq<JournalBlock>,
@@ -49,13 +51,19 @@ module JournalIntervals {
       journal': seq<Option<JournalBlock>>,
       indices: JournalInterval,
       newEntries: seq<JournalBlock>)
+  ensures JournalUpdate(journal, journal', indices, newEntries)
+      ==> 
+    && ValidJournal(journal)
+    && ValidJournal(journal')
+    && ValidJournalInterval(indices)
+    && indices.len == |newEntries|
   {
     && ValidJournal(journal)
     && ValidJournal(journal')
     && ValidJournalInterval(indices)
     && indices.len == |newEntries|
     && (forall i | 0 <= i < |journal| ::
-        journal'[i] == CyclicSliceValue(journal, indices, newEntries, i))
+        journal'[i] == CyclicSpliceValue(journal, indices, newEntries, i))
   }
 
   predicate InCyclicRange(i: int, indices: JournalInterval)
@@ -92,5 +100,241 @@ module JournalIntervals {
       Some(JournalInterval(0, 
           len - (NumJournalBlocks() as int - start)))
 
+  }
+
+  predicate subinterval(a: JournalInterval, b: JournalInterval)
+  {
+    || (a.start >= b.start && a.start + a.len <= b.start + b.len)
+    || (a.start + NumJournalBlocks() as int >= b.start
+        && a.start + NumJournalBlocks() as int + a.len <= b.start + b.len)
+  }
+
+  predicate journalIntervalOverlap(a: JournalInterval, b: JournalInterval)
+  requires ContiguousJournalInterval(a)
+  requires ContiguousJournalInterval(b)
+  {
+    && a.start + a.len > b.start
+    && b.start + b.len > a.start
+  }
+
+  predicate journalCyclicIntervalOverlap(a: JournalInterval, b: JournalInterval)
+  requires ValidJournalInterval(a)
+  requires ValidJournalInterval(b)
+  {
+    if a.start + a.len > NumJournalBlocks() as int then (
+      if b.start + b.len > NumJournalBlocks() as int then
+        true
+      else
+        || journalIntervalOverlap(JournalInterval(a.start, NumJournalBlocks() as int - a.start), b)
+        || journalIntervalOverlap(JournalInterval(0, a.len - (NumJournalBlocks() as int - a.start)), b)
+    ) else (
+      if b.start + b.len > NumJournalBlocks() as int then
+        || journalIntervalOverlap(JournalInterval(b.start, NumJournalBlocks() as int - b.start), a)
+        || journalIntervalOverlap(JournalInterval(0, b.len - (NumJournalBlocks() as int - b.start)), a)
+      else
+        journalIntervalOverlap(a, b)
+    )
+  }
+
+  function {:opaque} CyclicSlice<T>(s: seq<T>, interval: JournalInterval) : seq<T>
+  requires |s| == NumJournalBlocks() as int
+  requires 0 <= interval.start < NumJournalBlocks() as int
+  requires 0 <= interval.len <= NumJournalBlocks() as int
+  {
+    if interval.start + interval.len <= NumJournalBlocks() as int then
+      s[interval.start .. interval.start + interval.len]
+    else
+      s[interval.start ..] +
+        s[.. interval.start + interval.len - NumJournalBlocks() as int]
+  }
+
+  predicate fullRange(s: seq<Option<JournalBlock>>)
+  {
+    forall i | 0 <= i < |s| :: s[i].Some?
+  }
+
+  function concatFold(s: seq<Option<JournalBlock>>) : (res : seq<JournalBlock>)
+  requires fullRange(s)
+  ensures |res| == |s|
+  ensures forall i | 0 <= i < |s| :: Some(res[i]) == s[i]
+  {
+    if s == [] then [] else
+      concatFold(DropLast(s)) + [Last(s).value]
+  }
+
+  protected predicate Disk_HasJournalRange(journal: seq<Option<JournalBlock>>, interval: JournalInterval)
+  requires ValidJournalInterval(interval)
+  {
+    && |journal| == NumJournalBlocks() as int
+    && var slice := CyclicSlice(journal, interval);
+    && fullRange(slice)
+  }
+
+  protected function Disk_JournalRange(journal: seq<Option<JournalBlock>>, interval: JournalInterval) : JournalRange
+  requires ValidJournalInterval(interval)
+  requires Disk_HasJournalRange(journal, interval)
+  {
+    var slice := CyclicSlice(journal, interval);
+    concatFold(slice)
+  }
+
+  protected predicate Disk_HasJournal(
+      journal: seq<Option<JournalBlock>>, interval: JournalInterval)
+  requires ValidJournalInterval(interval)
+  {
+    && Disk_HasJournalRange(journal, interval)
+    && parseJournalRange(Disk_JournalRange(journal, interval)).Some?
+  }
+
+  protected function Disk_Journal(
+      journal: seq<Option<JournalBlock>>, interval: JournalInterval) : seq<JournalEntry>
+  requires ValidJournalInterval(interval)
+  requires Disk_HasJournal(journal, interval)
+  {
+    parseJournalRange(Disk_JournalRange(journal, interval)).value
+  }
+
+  lemma Disk_Journal_empty(
+      journal: seq<Option<JournalBlock>>, start: int)
+  requires ValidJournalInterval(JournalInterval(start, 0))
+  requires |journal| == NumJournalBlocks() as int
+  ensures Disk_HasJournal(journal, JournalInterval(start, 0))
+  ensures Disk_Journal(journal, JournalInterval(start, 0)) == []
+  {
+    reveal_CyclicSlice();
+    parseJournalRangeEmpty();
+  }
+
+  function Endpoint(interval: JournalInterval) : int
+  {
+    if interval.start + interval.len <= NumJournalBlocks() as int then
+      interval.start + interval.len
+    else
+      interval.start + interval.len - NumJournalBlocks() as int
+  }
+
+  function concatIntervals(a: JournalInterval, b: JournalInterval) : JournalInterval
+  requires Endpoint(a) == b.start
+  {
+    JournalInterval(a.start, a.len + b.len)
+  }
+
+  lemma Disk_Journal_preserves(
+      journal: seq<Option<JournalBlock>>,
+      journal': seq<Option<JournalBlock>>,
+      interval: JournalInterval,
+      interval_write: JournalInterval,
+      jr: JournalRange)
+  requires ValidJournalInterval(interval)
+  requires ValidJournalInterval(interval_write)
+  requires JournalUpdate(journal, journal', interval_write, jr)
+  requires Disk_HasJournal(journal, interval)
+  requires !journalCyclicIntervalOverlap(interval, interval_write)
+
+  ensures Disk_HasJournal(journal', interval)
+  ensures Disk_Journal(journal, interval)
+      == Disk_Journal(journal', interval)
+  {
+    var c1 := CyclicSlice(journal, interval);
+    var c2 := CyclicSlice(journal', interval);
+
+    assert c1 == c2 by {
+      reveal_CyclicSlice();
+      reveal_JournalUpdate();
+    }
+  }
+
+  lemma Disk_Journal_append(
+      journal: seq<Option<JournalBlock>>,
+      journal': seq<Option<JournalBlock>>,
+      interval: JournalInterval,
+      interval_write: JournalInterval,
+      jr: JournalRange)
+  requires ValidJournalInterval(interval)
+  requires JournalUpdate(journal, journal', interval_write, jr)
+  requires Disk_HasJournal(journal, interval)
+  requires parseJournalRange(jr).Some?
+  requires interval.len + |jr| <= NumJournalBlocks() as int
+  requires interval_write.start == Endpoint(interval)
+  ensures Disk_HasJournal(journal', concatIntervals(interval, interval_write))
+  ensures Disk_Journal(journal', concatIntervals(interval, interval_write))
+      == Disk_Journal(journal, interval) + parseJournalRange(jr).value
+  {
+    var interval' := concatIntervals(interval, interval_write);
+
+    var slice := CyclicSlice(journal, interval);
+    var slice' := CyclicSlice(journal', interval');
+
+    forall i | 0 <= i < |slice'|
+    ensures slice'[i].Some?
+    {
+      reveal_CyclicSlice();
+      reveal_JournalUpdate();
+      if i < interval.len {
+        if interval.start + i < NumJournalBlocks() as int {
+          calc {
+            slice[i];
+            journal[i + interval.start];
+            journal'[i + interval.start];
+            slice'[i];
+          }
+        } else {
+          calc {
+            slice[i];
+            slice'[i];
+          }
+        }
+        assert slice'[i].Some?;
+      } else {
+        assert slice'[i].Some?;
+      }
+    }
+
+    assert fullRange(slice');
+
+    var a := concatFold(slice');
+    var b := concatFold(slice) + jr;
+
+    assert |a| == |b| by { reveal_CyclicSlice(); }
+
+    forall i | 0 <= i < |a|
+    ensures a[i] == b[i]
+    {
+      reveal_CyclicSlice();
+      reveal_JournalUpdate();
+      if i < interval.len {
+        if interval.start + i < NumJournalBlocks() as int {
+          calc {
+            slice[i];
+            journal[i + interval.start];
+            journal'[i + interval.start];
+            slice'[i];
+          }
+        } else {
+          calc {
+            slice[i];
+            slice'[i];
+          }
+        }
+      } else {
+      }
+    }
+
+    assert Disk_HasJournalRange(journal', concatIntervals(interval, interval_write));
+    assert Disk_JournalRange(journal', concatIntervals(interval, interval_write))
+      == Disk_JournalRange(journal, interval) + jr;
+    parseJournalRangeAdditive(Disk_JournalRange(journal, interval), jr);
+  }
+
+  lemma Disk_Journal_Read(
+      journal: seq<Option<JournalBlock>>,
+      interval: JournalInterval)
+  requires ContiguousJournalInterval(interval)
+  requires Disk_HasJournalRange(journal, interval)
+  requires parseJournalRange(journal, Disk_JournalRange(journal, interval)).Some?
+  ensures Disk_HasJournal(journal, interval)
+  ensures Disk_Journal(journal, interval)
+      == parseJournalRange(Disk_JournalRange(journal, interval)).value
+  {
   }
 }
