BlockCacheSystem/Coupler.i.dfy
@@ -1,0 +1,66 @@
+module Coupler {
+
+  // HIgh level thing
+
+  datatype VersionedMap = VersionedMap(
+    states: seq<MapSpec>,
+    persistentIndex: Version,
+    syncReqs: map<SyncId, Version>
+  )
+
+  datatype VersionedMapStep =
+      | Write
+      | Crash
+      | Sync
+
+  // Journaloo
+
+  datatype Journaloo = Journaloo(
+    states: seq<MapSpec>,
+    persistentJournalIndex: Version,
+    persistentGraphIndex: Version,
+    frozenGraphIndex: Option<Version>,
+    frozenIndirectionTableLoc: Location,
+    persistentIndirectionTableLoc: Location,
+    syncReqs: map<SyncId, Version>
+  )
+
+  datatype JournalooStep =
+    | Write
+    | Crash // forget frozen stuff
+    | AdvanceJournal // persistentJournalIndex gets bigger
+    | NoOp
+    | Freeze // frozenIndex := |states|
+    | FrozenReadyToWrite // initialize frozenIndirectionTableLoc
+    | TruncateDone // update persistentIndirectionTableLoc := frozenIndirectionTableLoc
+               // persistentIndex := frozenIndex
+               // frozenIndex := None
+               // frozenIndirectionTableLoc := None
+    | LearnLocation // 
+
+  datatype GraphKeeper = GraphKeeper(
+    disk: map<Location, Map> // size 2
+    ephemeralState: Map,
+    frozenState: Map,
+    persistentLoc: Location,
+    frozenLoc: Location,
+
+  datatype GraphKeeperStep =
+    | Write // Advances ephemeralState
+    | Crash // forget in-memory stuff
+    | Freeze // set frozenState := ephemeralState
+    | NoOp // internal stuff, writing out nodes etc
+    | WriteFrozenState // conjure frozenLoc and set disk[frozenLoc] := frozenState
+    | FrozenReadyToWrite // enabling condition: frozenLoc exists
+    | TruncateDone // update persisnteLoc := frozenLoc, frozenLoc := None
+
+
+  datatype CoordinatorOp = // like diskOp
+      | Write
+      | Crash
+      | JournalooInternal
+      | BlockCacheInternal
+      | Freeze
+      | FrozenReadyToWrite(loc: Location)
+      | SyncDone
+}
